lakefile.lean
@@ -37,7 +37,7 @@ lean_exe mlirnatural {
 
 -- NOTE: this must be 'm'mathlib, as indicated from:
 --  https://github.com/leanprover-community/mathlib4#using-mathlib4-as-a-dependency
-require mathlib from git "https://github.com/leanprover-community/mathlib4" @ "aeb2e01"
+require mathlib from git "https://github.com/leanprover-community/mathlib4" @ "2d79858b28b32cd41534b73f17315812b7f7fd5a"
 
 require Cli from git "https://github.com/mhuisi/lean4-cli.git" @ "nightly"
 
